add some results on contract morphisms, esp isomorphisms and embeddings.

execution/theories/ContractMorphisms.v
@@ -2,12 +2,19 @@
 
 From Coq Require Import Basics.
 From Coq Require Import ProofIrrelevance.
+From Coq Require Import List.
+From Coq Require Import String.
+From Coq Require Import FunctionalExtensionality.
 From ConCert.Execution Require Import Blockchain.
 From ConCert.Execution Require Import Serializable.
 From ConCert.Execution Require Import ResultMonad.
+From ConCert.Execution Require Import ContractSystems.
+From ConCert.Execution Require Import BuildUtils.
+
+Axiom todo : string -> forall {A}, A.
 
 (* some auxiliary functions *)
-Definition curry_fun3 {A B C D : Type} (f : A * B * C -> D) : A -> B -> C -> D :=
+Definition curry_fun3 {A B C D : Type} (f : A * B * C -> D) : A -> B -> C -> D := 
     fun (a : A) => fun (b : B) => fun (c : C) => f (a,b,c).
 Definition uncurry_fun3 {A B C D : Type} (f : A -> B -> C -> D) : A * B * C -> D :=
     fun (x : A * B * C) => 
@@ -487,6 +494,103 @@ Proof.
         rewrite iso_f2. rewrite (composition_id_cm_right g). exact iso_g2.
 Qed.
 
+
+(*  Results about isomorphisms 
+
+    The following results show that :
+
+    (1) deploying isomorphic contracts produces isomorphic environments, or a bisimulation of 
+        environments
+    (2) an equivalence of environments is preserved under ActionEvaluation, where equivalent actions 
+        are paired via the isomorphism of environments
+
+    Together, these results show that deploying isomorphic contracts results two separate chains, along with a bisimulation of chains. Functionally, then, the chains behave in equivalent ways.
+*)
+
+(* we define a (functional) equivalence of environments via a function : this is a bisimulation *)
+Definition EnvironmentBisimulation (e1 e2 : Environment) : Prop := 
+    todo "".
+
+(* every environment is a bisimulation of itself *)
+Lemma env_equiv_then_bisimulation:
+    forall e1 e2,
+    EnvironmentEquiv e1 e2 -> 
+    EnvironmentBisimulation e1 e2.
+Proof. Admitted.
+
+(* deploying isomorphic contracts preserves a bisimulation *)
+Definition isomorphic_contracts_to_bisimulation
+        { Setup Setup' Msg Msg' State State' Error Error' : Type }
+        `{Serializable Msg}  `{Serializable Setup}  `{Serializable State}  `{Serializable Error}
+        `{Serializable Msg'} `{Serializable Setup'} `{Serializable State'} `{Serializable Error'}
+        {C : Contract Setup Msg State Error} {C' : Contract Setup' Msg' State' Error'} : 
+    forall (f : ContractMorphism C C') (g : ContractMorphism C' C),
+    is_iso_cm f g -> 
+    (* start with equivalent, reachable environments *)
+    forall env1 env2, 
+    reachable env1 ->
+    reachable env2 ->
+    EnvironmentBisimulation env1 env2 -> 
+    forall env1' env2' act_deploy_C act_deploy_C' new_acts s s' amt,
+    (* the environment we get by deploying C  *)
+    ActionEvaluation env1 act_deploy_C env1' new_acts -> 
+        act_deploy_C.(act_body) = act_deploy amt C s ->
+    (* the environment we get by deploying C'  *)
+    ActionEvaluation env2 act_deploy_C' env2' new_acts -> 
+        act_deploy_C'.(act_body) = act_deploy amt C' s' ->
+    (* the setups are equivalent under the isomorphism *)
+    s = s' -> (* TODO *)
+    (* they are deployed to the same address *)
+    forall caddr caddr',
+        env_contracts env1'  caddr  = Some (C  : WeakContract) -> 
+        env_contracts env2' caddr' = Some (C' : WeakContract) ->
+        caddr = caddr' ->
+    (* they are deployed BY the same address (and origin) *)
+    act_deploy_C.(act_from) = act_deploy_C'.(act_from) ->
+    act_deploy_C.(act_origin) = act_deploy_C'.(act_origin) ->
+    (* the isomorphisms f and g lift to a bisimulation of env' and env'' *)
+    EnvironmentBisimulation env1' env2' := todo "".
+
+(* if C and C' are isomorphic, then deploying  *)
+Lemma iso_cm_then_iso_env_init 
+        { Setup Setup' Msg Msg' State State' Error Error' : Type }
+        `{Serializable Msg}  `{Serializable Setup}  `{Serializable State}  `{Serializable Error}
+        `{Serializable Msg'} `{Serializable Setup'} `{Serializable State'} `{Serializable Error'}
+        {C : Contract Setup Msg State Error} {C' : Contract Setup' Msg' State' Error'} : 
+    forall (f : ContractMorphism C C') (g : ContractMorphism C' C),
+    is_iso_cm f g -> 
+    (* for all reachable states *)
+    forall env, reachable env -> 
+    forall env' env'' act_deploy_C act_deploy_C' new_acts s amt,
+    (* the environment we get by deploying C  *)
+    ActionEvaluation env act_deploy_C  env'  new_acts -> 
+        act_deploy_C.(act_body)  = act_deploy amt C  s ->
+    (* the environment we get by deploying C'  *)
+    ActionEvaluation env act_deploy_C' env'' new_acts -> 
+        act_deploy_C'.(act_body) = act_deploy amt C' s ->
+    (* they are deployed to the same address *)
+    forall caddr caddr',
+        env_contracts env'  caddr  = Some (C  : WeakContract) -> 
+        env_contracts env'' caddr' = Some (C' : WeakContract) ->
+        caddr = caddr' ->
+    (* they are deployed BY the same address (and origin) *)
+    act_deploy_C.(act_from) = act_deploy_C'.(act_from) ->
+    act_deploy_C.(act_origin) = act_deploy_C'.(act_origin) ->
+    (* the two environments are equivalent *)
+    EnvironmentBisimulation env' env''.
+Proof. Admitted.
+(* get a witness that env bisimulates itself, apply function above *)
+
+Lemma act_preserves_equiv : 
+    forall bstate1  bstate2,  EnvironmentBisimulation bstate1 bstate2 -> 
+    forall bstate1' bstate2' act1 act2 new_acts,
+        ActionEvaluation bstate1 act1 bstate1' new_acts -> 
+        ActionEvaluation bstate2 act2 bstate2' new_acts -> 
+        (* the act should be equivalent, not identical *)
+        act1 = act2 -> (* TODO *)
+        EnvironmentBisimulation bstate1' bstate2'.
+Proof. Admitted.
+
 End Isomorphisms.
 
 
@@ -507,6 +611,44 @@ Definition is_inj_cm
     is_inj (recv_inputs  C C' (recv_cm f)) /\
     is_inj (recv_outputs C C' (recv_cm f)).
 
+(* results about monomorphisms *)
+(* an EMBEDDING of traces *)
+
+Definition embed_trace bstate bstate1 bstate2 :
+    ChainTrace bstate bstate1 -> ChainTrace bstate bstate2 := todo "".
+
+Definition trace_embedding 
+        { Setup Setup' Msg Msg' State State' Error Error' : Type }
+        `{Serializable Msg}  `{Serializable Setup}  `{Serializable State}  `{Serializable Error}
+        `{Serializable Msg'} `{Serializable Setup'} `{Serializable State'} `{Serializable Error'}
+        {C1 : Contract Setup Msg State Error} {C2 : Contract Setup' Msg' State' Error'} : 
+    forall (f : ContractMorphism C1 C2), 
+    is_inj_cm f -> 
+    (* start with a reachable state *)
+    forall bstate, reachable bstate -> 
+    (* compare deploying C vs C' *)
+    forall (bstate1 bstate2 : ChainState) act_deploy_C1 act_deploy_C2 new_acts s1 s2 amt1 amt2,
+    (* the environment we get by deploying C  *)
+    ActionEvaluation bstate act_deploy_C1 bstate1 new_acts -> 
+        act_deploy_C1.(act_body) = act_deploy amt1 C1  s1 ->
+    (* the environment we get by deploying C'  *)
+    ActionEvaluation bstate act_deploy_C2 bstate2 new_acts -> 
+        act_deploy_C2.(act_body) = act_deploy amt2 C2 s2 ->
+    (* they are deployed to the same address *)
+    forall caddr1 caddr2,
+        env_contracts bstate1 caddr1 = Some (C1 : WeakContract) -> 
+        env_contracts bstate2 caddr2 = Some (C2 : WeakContract) ->
+        caddr1 = caddr2 ->
+    (* they are deployed BY the same address (and origin) *)
+    act_deploy_C1.(act_from)   = act_deploy_C2.(act_from)   ->
+    act_deploy_C1.(act_origin) = act_deploy_C2.(act_origin) ->
+    (* any state reachable through bstate1 has a corresponding state reachable through bstate2 *)
+    forall bstate1', reachable_through bstate1 bstate1' ->
+    forall (trace1 : ChainTrace bstate bstate1'),
+    exists bstate2' (trace2 : ChainTrace bstate bstate2'),
+        reachable_through bstate2 bstate2' /\ 
+        trace2 = embed_trace bstate bstate1' bstate2' trace1.
+Proof. Admitted.
 
 End Monomorphisms.
 
@@ -529,6 +671,133 @@ Definition is_surj_cm
     is_surj (recv_inputs C C' (recv_cm f)) /\
     is_surj (recv_outputs C C' (recv_cm f)).
 
+(* TODO : Result about surjections : possibly about rectacts, splitting C into C + C' via a retract *)
+(*                                 : possibly about upgradeability too *)
+
 End Epimorphisms.
+
+
+Section TerminalContract.
+    Import ListNotations.
+    Set Nonrecursive Elimination Schemes.
+
+(** State *)
+Record Null_State := { null_state : unit }.
+
+(** Msg *)
+Inductive Null_Msg := 
+| null_msg (n : unit).
+
+(** Setup *)
+Definition Null_Setup := option unit.
+
+(* one canonical error message *)
+Definition Null_Error := unit.
+
+(** Init/Recv Functions *)
+Definition null_init 
+    (_ : Chain) 
+    (_ : ContractCallContext) 
+    (null_init : Null_Setup) : result Null_State Null_Error := 
+        match null_init with 
+        | Some _ => Ok {| null_state := tt |}
+        | None => Err tt
+        end.
+
+Definition null_recv
+    (_ : Chain) 
+    (_ : ContractCallContext) 
+    (_ : Null_State) 
+    (op_msg : option Null_Msg) : 
+    result (Null_State * list ActionBody) Null_Error := 
+        match op_msg with 
+        | Some _ => Ok ({| null_state := tt |}, [])
+        | None => Err tt
+        end.
+
+(** Derive [Serializable] instances for state and messages *)
+Global Instance Null_State_serializable : Serializable Null_State :=
+Derive Serializable Null_State_rect<Build_Null_State>.
+
+Global Instance Null_Msg_serializable : Serializable Null_Msg :=
+Derive Serializable Null_Msg_rect<null_msg>.
+
+(** the Terminal contract *)
+Definition null_contract : Contract Null_Setup Null_Msg Null_State Null_Error := 
+    build_contract null_init null_recv.
+
+(* prove that every contract has a morphism into the terminal contract *)
+Context 
+    { Setup Msg State Error : Type } 
+    `{Serializable Msg} `{Serializable Setup} `{Serializable State} `{Serializable Error}
+    { C : Contract Setup Msg State Error }.
+
+(* init morphisms *)
+Definition morph_init_i (x : Chain * ContractCallContext * Setup) : Chain * ContractCallContext * Null_Setup :=
+    let (x', s) := x in let (c, ctx) := x' in
+    match (C.(init) c ctx s) with 
+    | Ok  _ => (c, ctx, Some tt)
+    | Err _ => (c, ctx, None)
+    end.
+Definition morph_init_o (x : result State Error) : result Null_State Null_Error := 
+    match x with 
+    | Ok  _ => Ok {| null_state := tt |}
+    | Err _ => Err tt
+    end.
+Lemma null_init_commutes : init_morphs_commute C.(init) null_contract.(init) morph_init_i morph_init_o.
+Proof.
+    unfold init_morphs_commute. 
+    intro. destruct x as [x' s]. destruct x' as [c ctx]. simpl.
+    unfold uncurry_fun3. unfold null_init. unfold morph_init_o.
+    now destruct (init C c ctx s).
+Qed.
+
+(* recv morphisms *)
+Definition morph_recv_i (x : Chain * ContractCallContext * State * option Msg) : Chain * ContractCallContext * Null_State * option Null_Msg := 
+    let (x', op_msg) := x in
+    let (x'', st) := x' in 
+    let (c, ctx) := x'' in 
+    match (C.(receive) c ctx st op_msg) with 
+    | Ok  _ => (c, ctx, {| null_state := tt |}, (Some (null_msg tt)))
+    | Err _ => (c, ctx, {| null_state := tt |}, None)
+    end.
+Definition morph_recv_o (x : result (State * list ActionBody) Error) : result (Null_State * list ActionBody) Null_Error := 
+    match x with 
+    | Ok  _ => Ok ({| null_state := tt |}, [])
+    | Err _ => Err tt 
+    end.
+Lemma null_recv_commutes : recv_morphs_commute C.(receive) null_contract.(receive) morph_recv_i morph_recv_o.
+Proof.
+    unfold recv_morphs_commute. intro.
+    destruct x as [x' op_msg]. destruct x' as [x'' st]. destruct x'' as [c ctx]. simpl.
+    unfold uncurry_fun4. unfold null_recv. unfold morph_recv_o.
+    now destruct (receive C c ctx st op_msg).
+Qed.
+
+(* the terminal morphism *)
+Definition null_morphism : ContractMorphism C null_contract := 
+    let morph_init := {|
+        init_inputs   := morph_init_i ; 
+        init_outputs  := morph_init_o ;
+        init_commutes := null_init_commutes ;
+    |} in
+    let morph_recv := {|
+        recv_inputs   := morph_recv_i ;
+        recv_outputs  := morph_recv_o ; 
+        recv_commutes := null_recv_commutes ;
+    |} in {| 
+        cm_init := morph_init ; 
+        cm_recv := morph_recv ;
+    |}.
+
+(* TODO: this is more nuanced *)
+Lemma null_morphism_unique : forall (f : ContractMorphism C null_contract), f = null_morphism.
+Proof. 
+    intro. apply is_eq_cm; try apply is_eq_cm_init; try apply is_eq_cm_recv; apply functional_extensionality; intro.
+    -   destruct x as [x' s]. destruct x' as [c ctx].
+        admit.
+    -   destruct x. Admitted.
+
+End TerminalContract.
 
 End ContractMorphisms.
